Examples.lean
@@ -12,6 +12,8 @@ import Examples.Language.Scalar
 import Examples.Language.ScalarCompiled
 import Examples.Language.Traversal
 import Examples.Language.TraversalCompiled
+import Examples.Language.TraversalComposition
+import Examples.Language.TraversalCompositionCompiled
 import Examples.Ram.AmortizedClear
 import Examples.Ram.Arithmetic
 import Examples.Ram.ArrayArguments
